Move OWGCounter to SteelSel

pulse/examples/steel/OWGCounterInv.fst
@@ -29,17 +29,17 @@ module G = FStar.Ghost
 
 open Steel.Memory
 open Steel.FractionalPermission
-open Steel.Reference
-open Steel.SpinLock
+open Steel.SelReference
+open Steel.SelSpinLock
 
-open Steel.Effect.Atomic
-open Steel.Effect
+open Steel.SelEffect.Atomic
+open Steel.SelEffect
 
-module R = Steel.Reference
+module R = Steel.SelReference
 module P = Steel.FractionalPermission
-module A = Steel.Effect.Atomic
+module A = Steel.SelEffect.Atomic
 
-open Steel.DisposableInvariant
+open Steel.SelDisposableInvariant
 
 #set-options "--using_facts_from '* -FStar.Tactics -FStar.Reflection' --fuel 0 --ifuel 0 --ide_id_info_off"
 
@@ -48,26 +48,26 @@ open Steel.DisposableInvariant
 (**** A few wrappers over library functions ****)
 
 let ghost_gather (#uses:inames) (v1 #v2:G.erased int) (r:ghost_ref int)
-  : SteelGhost unit uses
+  : SteelSelGhost unit uses
       (ghost_pts_to r (P.half_perm full_perm) v1 `star`
        ghost_pts_to r (P.half_perm full_perm) v2)
       (fun _ -> ghost_pts_to r full_perm v1)
       (fun _ -> True)
       (fun _ _ _ -> v1 == v2)
-  = ghost_gather #_ #_ #_ #_ #v1 #v2 r;
+  = ghost_gather_pt #_ #_ #_ #_ #v1 #v2 r;
     ()
 
 let ghost_share (#uses:inames) (v1 #v2:G.erased int) (r:ghost_ref int)
-  : SteelGhost unit uses
+  : SteelSelGhost unit uses
       (ghost_pts_to r full_perm v1)
       (fun _ -> ghost_pts_to r (P.half_perm full_perm) v1 `star`
              ghost_pts_to r (P.half_perm full_perm) v2)
       (fun _ -> v1 == v2)
       (fun _ _ _ -> True)
-  = ghost_share #_ #_ #_ #v1 r; ()
+  = ghost_share_pt #_ #_ #_ #v1 r; ()
 
-let gather_invariant (#p:slprop) (#uses:inames) (i:inv p)
-  : SteelGhostT unit uses
+let gather_invariant (#p:vprop) (#uses:inames) (i:inv p)
+  : SteelSelGhostT unit uses
       (active (P.half_perm full_perm) i `star` active (P.half_perm full_perm) i)
       (fun _ -> active full_perm i)
   = gather #_ #(P.half_perm full_perm) #(P.half_perm full_perm) #_ i; ()
@@ -79,15 +79,15 @@ let gather_invariant (#p:slprop) (#uses:inames) (i:inv p)
  *)
 inline_for_extraction
 let with_invariant (#a:Type)
-                   (#fp:slprop)
-                   (#fp':a -> slprop)
-                   (#p:slprop)
+                   (#fp:vprop)
+                   (#fp':a -> vprop)
+                   (#p:vprop)
                    (#perm:_)
                    (i:inv p)
-                   ($f:unit -> SteelAtomicT a (Set.singleton (Ghost.reveal (name i)))
+                   ($f:unit -> SteelSelAtomicT a (Set.singleton (Ghost.reveal (name i)))
                                              (p `star` fp)
                                              (fun x -> p `star` fp' x))
-  : SteelT a (active perm i `star` fp) (fun x -> active perm i `star` fp' x)
+  : SteelSelT a (active perm i `star` fp) (fun x -> active perm i `star` fp' x)
   = assert (Set.equal (Set.singleton (Ghost.reveal (name i))) (set_add (name i) Set.empty));
     with_invariant i f
 
@@ -97,6 +97,8 @@ let with_invariant (#a:Type)
  * The invariant holds half permission for the ghost refs and full perm for
  *   the counter, with an assertion relating their contents
  *)
+
+let half_perm = P.half_perm full_perm
 
 [@@ __reduce__]
 let inv_pred (r:ref int) (r1 r2:ghost_ref int) =
@@ -109,31 +111,55 @@ let inv_pred (r:ref int) (r1 r2:ghost_ref int) =
  * The h_exists slprop that the invariant protects
  *)
 [@@ __reduce__]
-let inv_slprop (r:ref int) (r1 r2:ghost_ref int) : slprop =
+let inv_slprop (r:ref int) (r1 r2:ghost_ref int) : vprop =
   h_exists (inv_pred r r1 r2)
 
 (*
  * A helper lemma to show that in the inv slprop the ghost refs commute with equiv
  *)
-#push-options "--warn_error -271"
+#push-options "--warn_error -271 --fuel 1"
 let inv_equiv_lemma (r:ref int) (r1 r2:ghost_ref int)
   : Lemma (inv_slprop r r1 r2 `equiv` inv_slprop r r2 r1)
           [SMTPat (inv_slprop r r1 r2)]
-  = let aux (r:ref int) (r1 r2:ghost_ref int) (m:mem)
+  =   let aux (r:ref int) (r1 r2:ghost_ref int) (m:mem)
       : Lemma
-          (requires interp (inv_slprop r r1 r2) m)
-          (ensures interp (inv_slprop r r2 r1) m)
+          (requires interp (hp_of (inv_slprop r r1 r2)) m)
+          (ensures interp (hp_of (inv_slprop r r2 r1)) m)
           [SMTPat ()]
-      = let w : G.erased (G.erased int & G.erased int) = id_elim_exists (inv_pred r r1 r2) m in
-        assert ((ghost_pts_to r1 (P.half_perm full_perm) (snd (snd w, fst w)) `star`
-                 ghost_pts_to r2 (P.half_perm full_perm) (fst (snd w, fst w)) `star`
-                 pts_to r full_perm (G.hide (G.reveal (fst (snd w, fst w)) + G.reveal (snd (snd w, fst w))))) `equiv`
-                (ghost_pts_to r2 (P.half_perm full_perm) (fst (snd w, fst w)) `star`
-                 ghost_pts_to r1 (P.half_perm full_perm) (snd (snd w, fst w)) `star`
-                 pts_to r full_perm (G.hide (G.reveal (fst (snd w, fst w)) + G.reveal (snd (snd w, fst w)))))) by Steel.Memory.Tactics.canon ();
+      = assert (
+          Steel.Memory.h_exists #(G.erased int & G.erased int) (fun x -> hp_of (inv_pred r r1 r2 x)) ==
+          h_exists_sl #(G.erased int & G.erased int) (inv_pred r r1 r2))
+          by (FStar.Tactics.norm [delta_only [`%h_exists_sl]]);
 
-        intro_h_exists (snd w, fst w) (inv_pred r r2 r1) m in
-    ()
+
+        let w : G.erased (G.erased int & G.erased int) = id_elim_exists (fun x -> hp_of (inv_pred r r1 r2 x)) m in
+
+        assert ((ghost_pts_to r1 half_perm (snd (snd w, fst w)) `star`
+                 ghost_pts_to r2 half_perm (fst (snd w, fst w)) `star`
+                 pts_to r full_perm (G.hide (G.reveal (fst (snd w, fst w)) + G.reveal (snd (snd w, fst w))))) `equiv`
+                (ghost_pts_to r2 half_perm (fst (snd w, fst w)) `star`
+                 ghost_pts_to r1 half_perm (snd (snd w, fst w)) `star`
+                 pts_to r full_perm (G.hide (G.reveal (fst (snd w, fst w)) + G.reveal (snd (snd w, fst w)))))) by (FStar.Tactics.norm [delta_attr [`%__steel_reduce__]]; canon' false (`true_p) (`true_p));
+
+        reveal_equiv
+          (ghost_pts_to r1 half_perm (snd (snd w, fst w)) `star`
+                 ghost_pts_to r2 half_perm (fst (snd w, fst w)) `star`
+                 pts_to r full_perm (G.hide (G.reveal (fst (snd w, fst w)) + G.reveal (snd (snd w, fst w)))))
+          (ghost_pts_to r2 half_perm (fst (snd w, fst w)) `star`
+                 ghost_pts_to r1 half_perm (snd (snd w, fst w)) `star`
+                 pts_to r full_perm (G.hide (G.reveal (fst (snd w, fst w)) + G.reveal (snd (snd w, fst w)))));
+
+        assert (interp (hp_of (inv_pred r r2 r1 (snd w, fst w))) m);
+
+        intro_h_exists (snd w, fst w) (fun x -> hp_of (inv_pred r r2 r1 x)) m;
+        assert (interp (Steel.Memory.h_exists (fun x -> hp_of (inv_pred r r2 r1 x))) m);
+
+        assert (
+          Steel.Memory.h_exists #(G.erased int & G.erased int) (fun x -> hp_of (inv_pred r r2 r1 x)) ==
+          h_exists_sl #(G.erased int & G.erased int) (inv_pred r r2 r1))
+          by (FStar.Tactics.norm [delta_only [`%h_exists_sl]]) in
+
+  reveal_equiv (inv_slprop r r1 r2) (inv_slprop r r2 r1)
 #pop-options
 
 
@@ -144,7 +170,7 @@ let incr (n:G.erased int) = G.elift1 (fun (n:int) -> n + 1) n
  * We assume an atomic increment operation for int refs
  *)
 assume val incr_atomic (#uses:inames) (#v:G.erased int) (r:ref int)
-  : SteelAtomicT unit uses
+  : SteelSelAtomicT unit uses
       (pts_to r full_perm v)
       (fun _ -> pts_to r full_perm (incr v))
 
@@ -155,7 +181,7 @@ assume val incr_atomic (#uses:inames) (#v:G.erased int) (r:ref int)
  *   and we return the same permissions with the incremented contents
  *)
 let incr_ghost_contrib (#uses:inames) (#v1 #v2:G.erased int) (r:ghost_ref int)
-  : SteelGhost unit uses
+  : SteelSelGhost unit uses
       (ghost_pts_to r (P.half_perm full_perm) v1 `star`
        ghost_pts_to r (P.half_perm full_perm) v2)
       (fun _ -> ghost_pts_to r (P.half_perm full_perm) (incr v1) `star`
@@ -163,7 +189,7 @@ let incr_ghost_contrib (#uses:inames) (#v1 #v2:G.erased int) (r:ghost_ref int)
       (fun _ -> True)
       (fun _ _ _ -> v1 == v2)
   = ghost_gather v1 r;
-    ghost_write r (incr v1);
+    ghost_write_pt r (incr v1);
     ghost_share (incr v1) r
 
 (*
@@ -185,7 +211,7 @@ inline_for_extraction
 let incr_with_inv_slprop
   (r:ref int) (r_mine r_other:ghost_ref int) (n_ghost:G.erased int) (b:bool) (name:Ghost.erased iname)
   ()
-  : SteelAtomicT unit (Set.singleton (Ghost.reveal name))
+  : SteelSelAtomicT unit (Set.singleton (Ghost.reveal name))
       (inv_slprop_conditional r r_mine r_other b
        `star`
        ghost_pts_to r_mine (P.half_perm full_perm) n_ghost)
@@ -194,16 +220,17 @@ let incr_with_inv_slprop
        `star`
        ghost_pts_to r_mine (P.half_perm full_perm) (incr n_ghost))
   = //get inv_slprop in the context
-    change_slprop (inv_slprop_conditional _ _ _ _)
-                  (inv_slprop _ _ _) (fun _ -> ());
-    let w : G.erased (G.erased int & G.erased int) = witness_h_exists () in
+    rewrite_slprop (inv_slprop_conditional _ _ _ _)
+                   (inv_slprop _ _ _) (fun _ -> Classical.forall_intro_2 reveal_equiv);
+    let w : G.erased (G.erased int & G.erased int) = witness_exists () in
     incr_atomic r;
     incr_ghost_contrib #_ #n_ghost #(fst w) r_mine;
 
     //restore inv_slprop, by first writing r to a form expected by the invariant
     intro_exists (incr (fst w), snd w) (inv_pred r r_mine r_other);
-    change_slprop (inv_slprop _ _ _)
-                  (inv_slprop_conditional _ _ _ _) (fun _ -> ())
+    rewrite_slprop (inv_slprop _ _ _)
+                   (inv_slprop_conditional _ _ _ _)
+                   (fun _ -> Classical.forall_intro_2 reveal_equiv)
 
 (*
  * A with_invariant wrapper over incr_with_inv_slprop
@@ -213,7 +240,7 @@ let incr_with_invariant
   (r:ref int) (r_mine r_other:ghost_ref int) (n_ghost:G.erased int) (b:bool)
   (i:inv (inv_slprop_conditional r r_mine r_other b))
   ()
-  : SteelT unit
+  : SteelSelT unit
       (active (P.half_perm full_perm) i `star` ghost_pts_to r_mine (P.half_perm full_perm) n_ghost)
       (fun _ -> active (P.half_perm full_perm) i `star` ghost_pts_to r_mine (P.half_perm full_perm) (incr n_ghost))
   = with_invariant i
@@ -223,16 +250,16 @@ let incr_with_invariant
  * The main thread
  *)
 let incr_main (#v:G.erased int) (r:ref int)
-  : SteelT unit
+  : SteelSelT unit
       (pts_to r full_perm v)
       (fun _ -> pts_to r full_perm (v + 2))
   = //allocate the two ghost refs
-    let r1 = ghost_alloc 0 in
-    let r2 = ghost_alloc v in
+    let r1 = ghost_alloc_pt 0 in
+    let r2 = ghost_alloc_pt v in
 
     //split their permissions
-    R.ghost_share r1;
-    R.ghost_share r2;
+    R.ghost_share_pt r1;
+    R.ghost_share_pt r2;
 
     //create the invariant
 
@@ -250,7 +277,8 @@ let incr_main (#v:G.erased int) (r:ref int)
     //gather back the invariant and dispose it
     gather_invariant i; dispose i;
 
-    let _ = A.witness_h_exists () in
+    let _ = witness_exists () in
 
     ghost_gather (incr 0) r1; ghost_gather (incr v) r2;
-    drop_f ()
+    drop (ghost_pts_to r1 _ _);
+    drop (ghost_pts_to r2 _ _)
